GroupoidModel/Syntax/Typechecker/Synth.lean
@@ -2,30 +2,21 @@ import GroupoidModel.Syntax.Typechecker.Equate
 
 open Qq
 
-partial def evalTp' (vΓ : Q(List Val)) (Γ : Q(Ctx)) (l : Q(Nat)) (T : Q(Expr))
-    (vΓwf : Q(TpEnvEqCtx $vΓ $Γ)) (ΓT : Q($Γ ⊢[$l] ($T))) :
-    Lean.MetaM ((v : Q(Val)) × Q(ValEqTp $Γ $l $v $T)) := do
-  -- TODO: WHNF `envOfTpEnv`?
-  let ⟨vT, vTeq_⟩ ← evalTp Γ q(envOfTpEnv $vΓ) q(Expr.bvar) Γ l T q(envOfTpEnv_wf $vΓwf) q($ΓT)
-  withHave vTeq_ fun vTeq => do
-  return ⟨vT, ← mkHaves #[vTeq] q(by as_aux_lemma =>
-    convert ($vTeq) using 1; autosubst
-  )⟩
-
-partial def lookup (Γ : Q(Ctx)) (i : Q(Nat)) :
-    Lean.MetaM ((A : Q(Expr)) × (l : Q(Nat)) × Q(Lookup $Γ $i $A $l)) :=
-  -- TODO: should this WHNF the weakening? See comment at `evalTp`.
-  match i, Γ with
-  | _, ~q([]) => throwError "bvar out of range: {i} ∉ {Γ}"
-  | ~q(.zero), ~q(($A, $l) :: $Γ') => do
-    return ⟨q(($A).subst Expr.wk), l, q(.zero $Γ' $A $l)⟩
-  | ~q(.succ $i), ~q(($B, $l') :: $Γ') => do
-    let ⟨A, l, lk⟩ ← lookup Γ' i
-    return ⟨q(($A).subst Expr.wk), l, q(($lk).succ $B $l')⟩
+-- partial def lookup (vΓ : Q(TpEnv)) (Γ : Q(Ctx)) (i : Q(Nat)) :
+--     Lean.MetaM ((vA : Q(Val)) × (l : Q(Nat)) × Q(Lookup $Γ $i $A $l)) :=
+--   -- TODO: should this WHNF the weakening? See comment at `evalTp`.
+--   sorry
+  -- match i, Γ with
+  -- | _, ~q([]) => throwError "bvar out of range: {i} ∉ {Γ}"
+  -- | ~q(.zero), ~q(($A, $l) :: $Γ') => do
+  --   return ⟨q(($A).subst Expr.wk), l, q(.zero $Γ' $A $l)⟩
+  -- | ~q(.succ $i), ~q(($B, $l') :: $Γ') => do
+  --   let ⟨A, l, lk⟩ ← lookup Γ' i
+  --   return ⟨q(($A).subst Expr.wk), l, q(($lk).succ $B $l')⟩
 
 mutual
 -- TODO: infer rather than check universe level?
-partial def checkTp (vΓ : Q(List Val)) (Γ : Q(Ctx)) (l : Q(Nat)) (T : Q(Expr))
+partial def checkTp (vΓ : Q(TpEnv)) (Γ : Q(Ctx)) (l : Q(Nat)) (T : Q(Expr))
     (vΓwf : Q(TpEnvEqCtx $vΓ $Γ)) :
     Lean.MetaM Q($Γ ⊢[$l] ($T)) :=
   match T with
@@ -36,7 +27,7 @@ partial def checkTp (vΓ : Q(List Val)) (Γ : Q(Ctx)) (l : Q(Nat)) (T : Q(Expr))
     withHave Awf_ fun Awf => do
     let ⟨vA, vAeq_⟩ ← evalTp' vΓ Γ k A vΓwf Awf
     withHave vAeq_ fun vAeq => do
-    let Bwf_ ← checkTp q($vA :: $vΓ) q(($A, $k) :: $Γ) k' B q(sorry)
+    let Bwf_ ← checkTp q(($vA, $k) :: $vΓ) q(($A, $k) :: $Γ) k' B q(($vΓwf).snoc $vAeq)
     withHave Bwf_ fun Bwf => do
     mkHaves #[leq, Awf, vAeq, Bwf] q(by as_aux_lemma =>
       cases ($leq)
@@ -49,7 +40,7 @@ partial def checkTp (vΓ : Q(List Val)) (Γ : Q(Ctx)) (l : Q(Nat)) (T : Q(Expr))
     withHave Awf_ fun Awf => do
     let ⟨vA, vAeq_⟩ ← evalTp' vΓ Γ k A vΓwf Awf
     withHave vAeq_ fun vAeq => do
-    let Bwf_ ← checkTp q($vA :: $vΓ) q(($A, $k) :: $Γ) k' B q(sorry)
+    let Bwf_ ← checkTp q(($vA, $k) :: $vΓ) q(($A, $k) :: $Γ) k' B q(($vΓwf).snoc $vAeq)
     withHave Bwf_ fun Bwf => do
     mkHaves #[leq, Awf, vAeq, Bwf] q(by as_aux_lemma =>
       cases ($leq)
@@ -67,91 +58,100 @@ partial def checkTp (vΓ : Q(List Val)) (Γ : Q(Ctx)) (l : Q(Nat)) (T : Q(Expr))
   | ~q(.el $a) => do
     let lmax_ ← ltNat l q(univMax)
     withHave lmax_ fun lmax => do
-    let awf_ ← checkTm vΓ Γ q($l + 1) a q(.univ $l) vΓwf q(.univ ($vΓwf).wf_ctx $lmax)
+    let awf_ ← checkTm vΓ Γ q($l + 1) a q(.univ $l) vΓwf
+      q(by as_aux_lemma => exact ⟨_, .univ ($vΓwf).wf_ctx $lmax⟩)
     withHave awf_ fun awf => do
-    mkHaves #[lmax, awf] q(WfTp.el $awf)
+    mkHaves #[lmax, awf] q(sorry)
   | _ =>
     throwError "not implemented: {Γ} ⊢[{l}]? {T}"
 
-partial def checkTm
-    (vΓ : Q(List Val)) (Γ : Q(Ctx)) (l : Q(Nat)) (t T : Q(Expr))
-    (vΓwf : Q(TpEnvEqCtx $vΓ $Γ)) (Twf : Q($Γ ⊢[$l] ($T))) :
-    Lean.MetaM Q(($Γ ⊢[$l] ($t) : $T)) := do
+partial def checkTm (vΓ : Q(TpEnv)) (Γ : Q(Ctx)) (l : Q(Nat)) (t : Q(Expr)) (vT : Q(Val))
+    (vΓwf : Q(TpEnvEqCtx $vΓ $Γ)) (vTwf : Q(∃ T, ValEqTp $Γ $l $vT T)) :
+    Lean.MetaM Q(∃ T, ValEqTp $Γ $l $vT T ∧ ($Γ ⊢[$l] ($t) : T)) := do
   /- We could do something more bidirectional,
   but all terms synthesize (thanks to extensive annotations). -/
-  withHave q(($Twf).wf_ctx) fun Γwf => do
-  let ⟨U, tU_⟩ ← synthTm vΓ Γ l t vΓwf
+  let ⟨vU, tU_⟩ ← synthTm vΓ Γ l t vΓwf
   withHave tU_ fun tU => do
-  let ⟨vT, vTeq_⟩ ← evalTp' vΓ Γ l T vΓwf q($Twf)
-  withHave vTeq_ fun vTeq => do
-  let ⟨vU, vUeq_⟩ ← evalTp' vΓ Γ l U vΓwf q(($tU).wf_tp)
-  withHave vUeq_ fun vUeq => do
-  let eq ← equateTp Γ l vU vT q(⟨_, $vUeq⟩) q(⟨_, $vTeq⟩)
-  mkHaves #[Γwf, tU, vTeq, vUeq] q(by as_aux_lemma =>
-    exact ($tU).conv <| ($eq).tp_uniq $vUeq $vTeq
+  let eq ← equateTp Γ l vU vT q(sorry) q(sorry)
+  mkHaves #[tU] q(by as_aux_lemma =>
+    sorry
+    -- exact ($tU).conv <| ($eq).tp_uniq $vUeq $vTeq
   )
 
-partial def synthTm (vΓ : Q(List Val)) (Γ : Q(Ctx)) (l : Q(Nat)) (t : Q(Expr))
+partial def synthTm (vΓ : Q(TpEnv)) (Γ : Q(Ctx)) (l : Q(Nat)) (t : Q(Expr))
     (vΓwf : Q(TpEnvEqCtx $vΓ $Γ)) :
-    Lean.MetaM ((T : Q(Expr)) × Q($Γ ⊢[$l] ($t) : $T)) :=
+    Lean.MetaM ((vT : Q(Val)) × Q(∃ T, ValEqTp $Γ $l $vT T ∧ ($Γ ⊢[$l] ($t) : T))) :=
   match t with
   | ~q(.bvar $i) => do
+    return ⟨q(sorry), q(sorry)⟩
     -- TODO: lookup in `vΓ` instead?
-    let ⟨A, m, lk_⟩ ← lookup Γ i
-    withHave lk_ fun lk => do
-    let lm_ ← equateNat l m
-    withHave lm_ fun lm => do
-    return ⟨A, ← mkHaves #[lk, lm] q(by as_aux_lemma =>
-      cases ($lm); exact WfTm.bvar ($vΓwf).wf_ctx $lk
-    )⟩
+    -- let ⟨A, m, lk_⟩ ← lookup Γ i
+    -- withHave lk_ fun lk => do
+    -- let lm_ ← equateNat l m
+    -- withHave lm_ fun lm => do
+    -- return ⟨A, ← mkHaves #[lk, lm] q(by as_aux_lemma =>
+    --   cases ($lm); exact WfTm.bvar ($vΓwf).wf_ctx $lk
+    -- )⟩
   | ~q(.lam $k $k' $A $b) => do
     let Awf_ ← checkTp vΓ Γ k A vΓwf
     withHave Awf_ fun Awf => do
     let ⟨vA, vAeq_⟩ ← evalTp' vΓ Γ k A vΓwf Awf
     withHave vAeq_ fun vAeq => do
-    let ⟨B, bB_⟩ ← synthTm q($vA :: $vΓ) q(($A, $k) :: $Γ) k' b q(sorry)
+    let ⟨vB, bB_⟩ ← synthTm q(($vA, $k) :: $vΓ) q(($A, $k) :: $Γ) k' b q(sorry)
     withHave bB_ fun bB => do
     let lmax_ ← equateNat l q(max $k $k')
     withHave lmax_ fun lmax => do
-    return ⟨q(.pi $k $k' $A $B), ← mkHaves #[Awf, vAeq, bB, lmax] q(by as_aux_lemma =>
-      cases ($lmax)
-      exact WfTm.lam $bB
+    -- TODO: oh no! What do we synth for the type of a lam?!??! need value-closures >.<
+    -- or readback. or storing the codomain type in `lam`.
+    -- or `coe` and bidir typechecking.
+    let vP : Q(Val) := q(.pi $k $k' $vA sorry)
+    return ⟨vP, ← mkHaves #[Awf, vAeq, bB, lmax] q(by as_aux_lemma =>
+      sorry
+      -- cases ($lmax)
+      -- exact WfTm.lam $bB
     )⟩
   | ~q(.app $k $k' $B $f $a) => do
     let lk'_ ← equateNat l k'
     withHave lk'_ fun lk' => do
-    let ⟨A, aA_⟩ ← synthTm vΓ Γ k a q($vΓwf)
-    withHave aA_ fun aA => do
-    -- TODO: if we synthesized NF types, then no need to eval here.
-    -- may need to do that to avoid WHNFing `subst` below.
-    let ⟨vA, vAeq_⟩ ← evalTp' vΓ Γ k A vΓwf q(sorry)
-    withHave vAeq_ fun vAeq => do
-    let Bwf_ ← checkTp q($vA :: $vΓ) q(($A, $k) :: $Γ) k' B q(sorry)
+    let ⟨vP, aP_⟩ ← synthTm vΓ Γ q(max $k $k') f q($vΓwf)
+    withHave aP_ fun aP => do
+    let ~q(.pi _ _ $vA _) := vP |
+      throwError "expected a Π-type but got{Lean.indentExpr vP}\nin the type of{Lean.indentExpr f}"
+    let awf_ ← checkTm vΓ Γ k a vA q($vΓwf) q(sorry)
+    withHave awf_ fun awf => do
+    let Bwf_ ← checkTp q(($vA, $k) :: $vΓ) q(sorry :: $Γ) k' B q(sorry)
     withHave Bwf_ fun Bwf => do
-    let fp_ ← checkTm vΓ Γ q(max $k $k') f q(.pi $k $k' $A $B) vΓwf q(.pi $Bwf)
-    withHave fp_ fun fp => do
-    let Ba : Q(Expr) := q(($B).subst ($a).toSb)
-    /- FIXME: computing a substitution here! should `eval`.
-    But if we evaluate, then we have to either:
-    - implement readback to get back an `Expr`; or
-    - return synthesized types in NF
-      which requires a lot more calls to `eval`. -/
-    let Ba' : Q(Expr) ← Lean.Meta.whnf Ba
-    have _ : $Ba' =Q $Ba := .unsafeIntro
-    return ⟨Ba', ← mkHaves #[lk', aA, vAeq, Bwf, fp] q(by as_aux_lemma =>
-      cases ($lk')
-      apply WfTm.app $fp $aA
+    let ⟨va, vaeq_⟩ ← evalTm' vΓ Γ k a q($vΓwf) q(sorry)
+    withHave vaeq_ fun vaeq => do
+    -- TODO: WHNF envOfTpEnv?
+    let ⟨vBa, vBaeq_⟩ ← evalTp Γ q($va :: envOfTpEnv $vΓ) q(($a).toSb) q(sorry :: $Γ) k' B
+      q(sorry) q(sorry)
+    return ⟨vBa, ← mkHaves #[lk', aP, awf, Bwf, vaeq] q(by as_aux_lemma =>
+      -- cases ($lk')
+      -- apply WfTm.app $fp $aA
+      sorry
     )⟩
-  | ~q(.pair ..) | ~q(.fst ..) | ~q(.snd ..) =>
+  | ~q(.pair $k $k' $B $t $u) => do
+    let lmax_ ← equateNat l q(max $k $k')
+    withHave lmax_ fun lmax => do
+    let ⟨vA, tA_⟩ ← synthTm vΓ Γ k t q($vΓwf)
+    withHave tA_ fun tA => do
+    let ⟨vU, uU_⟩ ← synthTm vΓ Γ k' u q($vΓwf)
+    withHave uU_ fun uU => do
+    -- Oh no! Don't have `A`! But don't need it :)
+    let vT : Q(Val) := q(.sigma $k $k' $vA (.mk_tp $Γ sorry sorry $B))
+    throwError "not implemented: {Γ} ⊢[{l}] {t} : ?"
+  | ~q(.fst ..) | ~q(.snd ..) =>
     throwError "not implemented: {Γ} ⊢[{l}] {t} : ?"
   | ~q(.code $A) => do
     -- TODO: WHNF `l`? See comment at `evalTp`.
-    let ~q(.succ $k) := l | throwError "abcd"
+    let ~q(.succ $k) := l | throwError "expected _+1, got{Lean.indentExpr l}"
     let lmax_ ← ltNat k q(univMax)
     withHave lmax_ fun lmax => do
     let Awf_ ← checkTp vΓ Γ k A vΓwf
     withHave Awf_ fun Awf => do
-    return ⟨q(.univ $k), ← mkHaves #[lmax, Awf] q(WfTm.code $lmax $Awf)⟩
+    let vU : Q(Val) := q(.univ $k)
+    return ⟨vU, ← mkHaves #[lmax, Awf] q(sorry)⟩
   | _ =>
     throwError "{t} is not a term in {Γ} ⊢[{l}] {t} : ?"
 end
